platform/cito/InvFacts.v
@@ -1,29 +1,37 @@
-Require Import Inv.
-Require Import Semantics.
-
 Set Implicit Arguments.
 
-Lemma make_triples_Word : forall pairs outs, length outs = length pairs -> map Word (make_triples pairs outs) = map fst pairs.
-  admit.
-Qed.
+Require Import ADT.
 
-Lemma make_triples_Word_ADTIn : forall pairs outs, length outs = length pairs -> map (fun x => (Word x, ADTIn x)) (make_triples pairs outs) = pairs.
-  admit.
-Qed.
+Module Make (Import E : ADT).
 
-Lemma make_triples_ADTIn : forall pairs outs, length outs = length pairs -> map ADTIn (make_triples pairs outs) = map snd pairs.
-  admit.
-Qed.
+  Require Import Inv.
+  Module Import InvMake := Make E.
+  Import SafeMake.SemanticsMake.
+  Import HeapMake.
 
-Lemma make_triples_length : forall pairs outs, length outs = length pairs -> length (make_triples pairs outs) = length pairs.
-  admit.
-Qed.
+  Lemma make_triples_Word : forall pairs outs, length outs = length pairs -> map Word (make_triples pairs outs) = map fst pairs.
+    admit.
+  Qed.
 
-Lemma heap_merge_store_out : 
-  forall h pairs outs, 
-    good_inputs h pairs -> 
-    let h1 := make_heap pairs in 
-    let triples := make_triples pairs outs in
-    heap_merge (heap_diff h h1) (fold_left store_out triples h1) = fold_left store_out triples h.
-  admit.
-Qed.
+  Lemma make_triples_Word_ADTIn : forall pairs outs, length outs = length pairs -> map (fun x => (Word x, ADTIn x)) (make_triples pairs outs) = pairs.
+    admit.
+  Qed.
+
+  Lemma make_triples_ADTIn : forall pairs outs, length outs = length pairs -> map ADTIn (make_triples pairs outs) = map snd pairs.
+    admit.
+  Qed.
+
+  Lemma make_triples_length : forall pairs outs, length outs = length pairs -> length (make_triples pairs outs) = length pairs.
+    admit.
+  Qed.
+
+  Lemma heap_merge_store_out : 
+    forall h pairs outs, 
+      good_inputs h pairs -> 
+      let h1 := make_heap pairs in 
+      let triples := make_triples pairs outs in
+      heap_merge (heap_diff h h1) (fold_left store_out triples h1) = fold_left store_out triples h.
+    admit.
+  Qed.
+
+End Make.
